

# Worksheet # 10

MATH 3160 – Complex Variables  
Miguel Gomez

Completed: November 16, 2025

## Problem 1

Use the Taylor series of  $\sin(z)$ ,  $\cos(z)$ , and  $e^z$  at  $z = 0$  to prove Euler's formula:

$$e^{iz} = \cos(z) + i \sin(z)$$

---

Using the known expression for the expansion of the exponential shown above:

$$\begin{aligned} e^x &= \sum_{n=0}^{\infty} \frac{x^n}{n!} \\ e^{iz} &= \sum_{n=0}^{\infty} \frac{(iz)^n}{n!} \\ &= 1 + \frac{(iz)^1}{1!} + \frac{(iz)^2}{2!} + \frac{(iz)^3}{3!} + \frac{(iz)^4}{4!} + \frac{(iz)^5}{5!} + \frac{(iz)^6}{6!} + \dots \\ &= 1 + i(z)^1 + i^2 \frac{(z)^2}{2!} + i^3 \frac{(z)^3}{3!} + i^4 \frac{(z)^4}{4!} + i^5 \frac{(z)^5}{5!} + i^6 \frac{(z)^6}{6!} + \dots \end{aligned}$$

The resulting pattern shows that we have  $i$  in many of the expressions, but we can reduce all the products of  $i$  with itself to the following.

$$\begin{aligned} i^0 &= i^4 = i^{4n} = 1 \\ i^1 &= i^5 = i^{4n+1} = i \\ i^2 &= i^6 = i^{4n+2} = -1 \\ i^3 &= i^7 = i^{4n+3} = -i \end{aligned}$$

This shows that the expansion can be reduced to either have a factor of  $i$  or not. Therefore, we can

reduce the expansion further:

$$\begin{aligned}
 &= 1 + i(z)^1 + (-1)\frac{(z)^2}{2!} - i\frac{(z)^3}{3!} + (1)\frac{(z)^4}{4!} + i\frac{(z)^5}{5!} - (1)\frac{(z)^6}{6!} + \dots \\
 &= 1 + i(z)^1 - \frac{(z)^2}{2!} - i\frac{(z)^3}{3!} + \frac{(z)^4}{4!} + i\frac{(z)^5}{5!} - (1)\frac{(z)^6}{6!} + \dots \\
 &= 1 - \frac{(z)^2}{2!} + \frac{(z)^4}{4!} - (1)\frac{(z)^6}{6!} + i(z)^1 - i\frac{(z)^3}{3!} + i\frac{(z)^5}{5!} \dots \\
 &= \left(1 - \frac{(z)^2}{2!} + \frac{(z)^4}{4!} - \frac{(z)^6}{6!} + \dots\right) + i \left((z)^1 - \frac{(z)^3}{3!} + \frac{(z)^5}{5!} \dots\right)
 \end{aligned}$$

The expansion of  $\sin(z)$  and  $\cos(z)$ :

$$\begin{aligned}
 \sin(z) &= \sum_{n=0}^{\infty} (-1)^n \frac{z^{2n+1}}{2n+1!} \\
 &= (z)^1 - \frac{(z)^3}{3!} + \frac{(z)^5}{5!} - \frac{(z)^7}{7!} + \dots \\
 \cos(z) &= \sum_{n=0}^{\infty} (-1)^n \frac{z^{2n}}{2n!} \\
 &= 1 - \frac{(z)^2}{2!} + \frac{(z)^4}{4!} - \frac{(z)^6}{6!} + \dots
 \end{aligned}$$

Notice how the  $\sin(z)$  and  $\cos(z)$  expansions are exactly what we see in the expression above when expanding out and grouping the expression of  $e^{iz}$

$$\begin{aligned}
 \therefore e^{iz} &= \sum_{n=0}^{\infty} (-1)^n \frac{z^{2n}}{2n!} + i \sum_{n=0}^{\infty} (-1)^n \frac{z^{2n+1}}{2n+1!} \\
 &= \cos(z) + i \sin(z)
 \end{aligned}$$

## Problem 2

Find  $f^{(10)}(3)$  for  $f(z)$  as given below. You can leave the answer in terms of powers, factorials, etc.

$$f(z) = \sum_{n=0}^{\infty} n^2 (z-3)^n$$


---

To do this, we can employ the following expressions:

$$\begin{aligned} f(z) &= \sum_{n=0}^{\infty} a_n (z - z_0)^n \\ f^{(n)}(z) &= n! a_n \\ a_n &= \frac{f^{(n)}(z_0)}{n!} \end{aligned}$$

So any term that would be present at the 10th derivative summation greater than  $n$  would disappear from being a constant or having a factor of  $(z-3)$ . Meaning we only get the final term being:

$$\begin{aligned} f^{(10)}(3) &= 10! a_n \\ a_n &= n^2 = 10^2 = 100 \\ \therefore f^{(10)}(3) &= 100 \cdot 10! \end{aligned}$$

### Problem 3

List the first four nonzero terms of the Taylor series for  $f(z) = \cos(3z + 2)$  centered at  $z = -\frac{2}{3}$ .

---

Here, we need to change the expression to look like  $a_n(z - z_0)$ :

$$\cos(3z + 2) = \cos\left(3\left(z + \frac{2}{3}\right)\right)$$

expanding this out with the expansion we showed before:

$$\begin{aligned}\cos(z) &= \sum_{n=0}^{\infty} (-1)^n \frac{z^{2n}}{2n!} \\ &= 1 - \frac{(z)^2}{2!} + \frac{(z)^4}{4!} - \frac{(z)^6}{6!} + \dots\end{aligned}$$

This is already the first four terms, we only need to replace the  $z$  with our expression:

$$1 - \frac{(3(z + \frac{2}{3}))^2}{2!} + \frac{(3(z + \frac{2}{3}))^4}{4!} - \frac{(3(z + \frac{2}{3}))^6}{6!}$$